common/Separation.v
@@ -852,7 +852,8 @@ Lemma external_call_parallel_rule:
   external_call ef ge vargs1 m1 t vres1 m1' ->
   m2 |= minjection j m1 ** globalenv_inject ge j ** P ->
   Val.inject_list j vargs1 vargs2 ->
-  exists w, forall t2, match_events cc_inject w t t2 ->
+  exists w, (exists t2, match_events_query cc_inject w t t2) /\
+  forall t2, match_events cc_inject w t t2 ->
   exists j' vres2 m2',
      external_call ef ge vargs2 m2 t2 vres2 m2'
   /\ Val.inject j' vres1 vres2
@@ -864,7 +865,8 @@ Proof.
   destruct SEP as (A & B & C). simpl in A.
   exploit external_call_mem_inject; eauto.
   eapply globalenv_inject_preserves_globals. eapply sep_pick1; eauto.
-  intros [w Hw]. exists w; intros t2 Ht2. specialize (Hw t2 Ht2).
+  intros (w & Hwq & Hw). exists w; split; eauto.
+  intros t2 Ht2. specialize (Hw t2 Ht2).
   destruct Hw as (j' & vres2 & m2' & CALL' & RES & INJ' & UNCH1 & UNCH2 & INCR & ISEP).
   assert (MAXPERMS: forall b ofs p,
             Mem.valid_block m1 b -> Mem.perm m1' b ofs Max p -> Mem.perm m1 b ofs Max p).
